Add first sketches of GM impl

code/experimental/he/Hacl.Impl.HE.GM.fst
@@ -9,9 +9,75 @@ open LowStar.Buffer
 open Lib.IntTypes
 open Lib.Buffer
 open Lib.PrintBuffer
+open Lib.Math.Algebra
 
-open Hacl.Impl.Bignum.Addition
-open Hacl.Impl.Bignum.Core
+open Hacl.Impl.Bignum
 
-val testfunc : lbuffer8 5ul -> lbuffer8 6ul
-let testfunc _ = admit()
+module S = Hacl.Spec.HE.GM
+
+// max 2^14 bits
+type bn_len_s = s:bn_len{v s <= 256}
+
+val to_fe:
+     #nLen:bn_len_s
+  -> n:lbignum nLen
+  -> a:lbignum nLen
+  -> res:lbignum nLen
+  -> Stack unit
+    (requires fun h ->
+       live h n /\ live h a /\ live h res /\
+       disjoint n res /\ disjoint a res /\
+       as_snat h n > 1)
+    (ensures fun h0 _ h1 ->
+       modifies1 res h0 h1 /\
+       as_snat h1 res = to_fe #(as_snat h0 n) (as_snat h0 a))
+let to_fe #nLen n a res = bn_remainder a n res
+
+val leg_symbol:
+     #nLen:bn_len_s
+  -> a:lbignum nLen
+  -> p:lbignum nLen
+  -> p_min_one:lbignum nLen
+  -> p_min_one_half:lbignum nLen
+  -> Stack Int32.t
+    (requires fun h ->
+       live h a /\ live h p /\ live h p_min_one /\ live h p_min_one_half /\
+       disjoint a p /\
+       as_snat h p > 1 /\
+       as_snat h p_min_one = as_snat h p - 1 /\
+       as_snat h p_min_one_half = as_snat h p_min_one / 2)
+    (ensures  fun h0 _ h1 ->
+       live h1 a /\ live h1 p /\ modifies0 h0 h1)
+let leg_symbol #nLen a p p_min_one p_min_one_half =
+  push_frame ();
+  let tmp = create nLen (uint 0) in
+  bn_modular_exp p a p_min_one_half tmp;
+  let res = if bn_is_equal p_min_one tmp then (-1l)
+            else (if eq_u64 (tmp.(0ul) &. uint 1) (uint 1) then 1l else 0l) in
+  pop_frame ();
+  res
+
+
+val encrypt:
+     #nLen:bn_len_s
+  -> n:lbignum nLen
+  -> y:lbignum nLen
+  -> m:bool
+  -> r:lbignum nLen
+  -> res:lbignum nLen
+  -> Stack unit
+    (requires fun h ->
+       live h n /\ live h y /\ live h r /\ live h res /\
+       disjoint n res /\ disjoint y res /\ disjoint r res /\
+       as_snat h n > 1)
+    (ensures fun h0 _ h1 ->
+       live h1 n /\ live h1 y /\ live h1 r /\ live h1 res /\
+       modifies1 res h0 h1)
+let encrypt #nLen n y m r res =
+  if m then bn_modular_mul n r r res else begin
+    push_frame ();
+    let r' = create nLen (uint 0) in
+    bn_modular_mul n r r res;
+    bn_modular_mul n r' y res;
+    pop_frame ()
+  end
