code/experimental/rsapss/Hacl.Impl.Bignum.Division.fst
@@ -58,6 +58,7 @@ let rec calc_bits_test #aLen a ind =
   if ind =. 0ul then 0ul else
   if bn_is_bit_set a ind then ind else calc_bits_test a (ind -! 1ul)
 
+// Returns the index of the highest bit set plus one.
 val calc_bits:
      #aLen:bn_len_strict
   -> a:lbignum aLen
@@ -66,62 +67,131 @@ val calc_bits:
     (ensures  fun h0 _ h1 -> modifies0 h0 h1 /\ h0 == h1 /\ live h1 a)
 let calc_bits #aLen a = calc_bits_test a (aLen *! 64ul -! 1ul)
 
-// res = a % n
-val bn_remainder:
-     #aLen:bn_len_strict
-  -> #modLen:bn_len_strict
+
+/// Copies the part that fits.
+val copy_fit:
+     #oLen:bn_len
+  -> #iLen:bn_len
+  -> o:lbignum oLen
+  -> i:lbignum iLen
+  -> Stack unit
+    (requires fun h -> live h o /\ live h i /\ disjoint i o)
+    (ensures fun h0 _ h1 -> live h1 o /\ live h1 i /\ modifies1 o h0 h1)
+let copy_fit #oLen #iLen o i =
+  if iLen >=. oLen
+  then copy o (sub i 0ul oLen)
+  else begin
+    copy (sub o 0ul iLen) i;
+    memset (sub o iLen (oLen -. iLen)) (uint 0) (oLen -. iLen)
+  end
+
+
+#reset-options "--z3rlimit 50 --max_fuel 0 --max_ifuel 0"
+
+
+// Central part of remainder, w/o it remainder verifies for ages.
+val bn_remainder_reduce:
+     #aLen:bn_len{ v aLen * 64 <= max_size_t }
+  -> #modLen:bn_len{ v modLen * 64 <= max_size_t }
   -> a:lbignum aLen
   -> mod:lbignum modLen
   -> res:lbignum modLen
+  -> realALen:bn_len{ v realALen <= v aLen }
+  -> diffBits:size_t
+  -> mod1Len:bn_len{v mod1Len = v modLen + (v diffBits / 64) + 1 /\ v mod1Len >= v realALen}
+  -> count:size_t
   -> Stack unit
-    (requires fun h -> live h a /\ live h mod /\ live h res)
+    (requires fun h ->
+     live h a /\ live h mod /\ live h res /\
+     disjoint res a /\ disjoint res mod /\ as_snat h mod > 1)
     (ensures fun h0 _ h1 ->
-        live h1 a /\ live h1 mod /\ live h1 res /\
-        modifies1 res h0 h1)
-let bn_remainder #aLen #modLen a mod res =
-  push_frame();
-
-  let modBits = calc_bits mod in
-  let aBits = calc_bits a in
-  let realALen = aBits /. 64ul in
-
-  if aBits >=. modBits then begin
-    assume (v aBits >= v modBits);
-    let diffBits = aBits -! modBits in // +1?
-    let modk = diffBits /. 64ul in
-    assume ((v modLen + v modk + 1) * 64 < max_size_t);
-    assume (v modLen + v modk + 1 > 0);
-    assume (v (modLen +! modk) + 1 > 0);
-    let mod1Len:bn_len = modLen +! modk +! 1ul in
-    // this push_frame() is required, because otherwise
-    // kremlin says it can't generate buffer allocation
-    // because of the variable length.
+     live h1 a /\ live h1 mod /\ live h1 res /\ modifies1 res h0 h1)
+let bn_remainder_reduce #aLen #modLen a mod res realALen diffBits mod1Len count =
     push_frame();
+
     let mod1 = create mod1Len (uint 0) in
     bn_lshift mod diffBits mod1;
-    assume (v mod1Len <= v aLen);
+
+    let mod2 = sub mod1 0ul realALen in
 
     let res1 = create aLen (uint 0) in
     copy (sub res1 0ul aLen) a;
 
-    assume (v diffBits + 1 < max_size_t);
-    bn_remainder_core res1 mod1 (diffBits +! 1ul);
+    bn_remainder_core res1 mod2 count;
 
-    copy res (sub res1 0ul modLen);
+    copy_fit res res1;
     pop_frame()
-  end
-  else
-  begin
-    // what's wrong???
-    if aLen >=. modLen
-    then (assert (v aLen >= v modLen); admit(); copy res (sub a 0ul modLen))
-    else (admit(); copy (sub res 0ul aLen) a)
+
+
+#reset-options "--z3rlimit 100 --max_fuel 1 --max_ifuel 0"
+
+// res = a % n
+val bn_remainder:
+     #aLen:bn_len{ v aLen * 64 <= max_size_t }
+  -> #modLen:bn_len{ v modLen * 64 <= max_size_t }
+  -> a:lbignum aLen
+  -> mod:lbignum modLen
+  -> res:lbignum modLen
+  -> Stack unit
+    (requires fun h ->
+       live h a /\ live h mod /\ live h res /\
+       disjoint res a /\ disjoint res mod /\ as_snat h mod > 1)
+    (ensures fun h0 _ h1 ->
+       live h1 a /\ live h1 mod /\ live h1 res /\ modifies1 res h0 h1 /\
+       as_snat h1 res = as_snat h0 a % as_snat h0 mod)
+let bn_remainder #aLen #modLen a mod res =
+  let h0 = FStar.HyperStack.ST.get () in
+
+  push_frame();
+
+  let modBits = calc_bits mod in
+  let aBits = calc_bits a in
+
+  if aBits =. 0ul then memset res (uint 0) modLen else
+  if modBits >. aBits then copy_fit res a
+  else begin
+    ne_lemma aBits 0ul;
+    assert (v aBits > 0);
+
+    let realALen = blocks aBits 64ul in
+    assume (v realALen <= v aLen); // always true
+
+    let maxLen:bn_len_strict = if aLen >=. modLen then aLen else modLen in
+    let diffBits = aBits -! modBits in
+    assume (v diffBits < 64 * v maxLen); // always true
+
+    let mod1Len:bn_len = begin
+        let modk = diffBits /. 64ul in
+        assert (v modLen + v modk + 1 <= 3 * v maxLen);
+        assert (3 * v maxLen <= max_size_t);
+        assert (v modLen + v modk + 1 <= max_size_t);
+        modLen +! modk +! 1ul
+      end in
+
+    let count:size_t = begin
+        assert (v diffBits + 1 <= 64 * v maxLen);
+        assert (64 * v maxLen <= max_size_t);
+        assert (v diffBits + 1 <= max_size_t);
+        (diffBits +! 1ul)
+    end in
+
+    // They are equal if modLen < realALen
+    assume (v mod1Len >= v realALen);
+
+    bn_remainder_reduce a mod res realALen diffBits mod1Len count
+
   end;
 
-  pop_frame()
+  pop_frame();
+
+  let h1 = FStar.HyperStack.ST.get () in
+  assume (as_snat h1 res = as_snat h0 a % as_snat h0 mod)
+
+
+#reset-options "--z3rlimit 50 --max_fuel 1 --max_ifuel 0"
 
 val bn_modular_add:
-     #len:bn_len_strict{(v len + 1) * 64 < max_size_t}
+     #len:bn_len{ (v len + 1) * 64 <= max_size_t}
   -> n:lbignum len
   -> a:lbignum len
   -> b:lbignum len
@@ -129,27 +199,21 @@ val bn_modular_add:
   -> Stack unit
     (requires fun h ->
        live h n /\ live h a /\ live h b /\ live h res /\
+       disjoint res a /\ disjoint res b /\ disjoint res n /\
        as_snat h n > 1)
     (ensures  fun h0 _ h1 ->
-         live h1 n /\ live h1 a /\ live h1 b /\ live h1 res /\
-         modifies (loc res) h0 h1 /\
-         (let n' = as_snat h0 n in
-         to_fe #n' (as_snat h1 res) = to_fe (as_snat h0 a) +% to_fe (as_snat h0 b)))
+       live h1 n /\ live h1 a /\ live h1 b /\ live h1 res /\
+       modifies (loc res) h0 h1 /\
+       as_snat h1 res = (as_snat h0 a + as_snat h0 b) % as_snat h0 n)
 let bn_modular_add #len n a b res =
-  let h0 = FStar.HyperStack.ST.get () in
-  push_frame ();
-  assert (v len < max_size_t);
+  push_frame();
   let res' = create (len +! 1ul) (uint 0) in
   bn_add_full a b res';
   bn_remainder res' n res;
-  pop_frame ();
-  let h1 = FStar.HyperStack.ST.get () in
-  assume (let n' = as_snat h0 n in
-          to_fe #n' (as_snat h1 res) =
-          to_fe (as_snat h0 a) +% to_fe (as_snat h0 b))
+  pop_frame()
 
 val bn_modular_mul:
-     #len:bn_len_strict{(v len + v len) * 64 < max_size_t}
+     #len:bn_len_strict{v len * 128 < max_size_t}
   -> n:lbignum len
   -> a:lbignum len
   -> b:lbignum len
@@ -157,20 +221,15 @@ val bn_modular_mul:
   -> Stack unit
     (requires fun h ->
        live h n /\ live h a /\ live h b /\ live h res /\
+       disjoint res a /\ disjoint res b /\ disjoint res n /\
        as_snat h n > 1)
     (ensures  fun h0 _ h1 ->
-         live h1 n /\ live h1 a /\ live h1 b /\ live h1 res /\
-         modifies (loc res) h0 h1 /\
-         (let n' = as_snat h0 n in
-         to_fe #n' (as_snat h1 res) = to_fe (as_snat h0 a) *% to_fe (as_snat h0 b)))
+       live h1 n /\ live h1 a /\ live h1 b /\ live h1 res /\
+       modifies (loc res) h0 h1 /\
+       as_snat h1 res = (as_snat h0 a * as_snat h0 b) % as_snat h0 n)
 let bn_modular_mul #len n a b res =
-  let h0 = FStar.HyperStack.ST.get () in
   push_frame ();
   let res' = create (len +! len) (uint 0) in
   bn_mul a b res';
   bn_remainder res' n res;
-  pop_frame ();
-  let h1 = FStar.HyperStack.ST.get () in
-  assume (let n' = as_snat h0 n in
-          to_fe #n' (as_snat h1 res) =
-          to_fe (as_snat h0 a) *% to_fe (as_snat h0 b))
+  pop_frame ()
