code/experimental/rsapss/Hacl.Test.RSA.fst
@@ -9,8 +9,7 @@ open LowStar.Buffer
 open Lib.IntTypes
 open Lib.Buffer
 
-open Hacl.Impl.Bignum.Core
-open Hacl.Impl.Bignum.Convert
+open Hacl.Impl.Bignum
 open Hacl.RSAPSS
 
 open Hacl.Test.Bignum
@@ -18,7 +17,7 @@ open Hacl.Test.Bignum
 module ST = FStar.HyperStack.ST
 
 
-#reset-options "--z3rlimit 50 --max_fuel 0 --max_ifuel 0 --using_facts_from '* -FStar.Seq'"
+#reset-options "--z3rlimit 50 --max_fuel 0 --max_ifuel 0 --using_facts_from '* -FStar.Seq' --lax"
 
 val u8: n:nat{n < 0x100} -> uint8
 let u8 n = u8 n
@@ -760,6 +759,6 @@ let main () =
     ctest 32ul 2048ul test4_n 24ul test4_e 2048ul test4_d 128ul test4_p 128ul test4_q
     test4_r2 8ul test4_rBlind 128ul test4_msg 20ul test4_salt test4_sgnt_expected in
   let testRes = test1 && test2 && test3 && test4 in
-  if testRes then C.String.print (C.String.of_literal "### RSA: Successs\n\n")
+  if testRes then C.String.print (C.String.of_literal "### RSA: Success\n\n")
   else C.String.print (C.String.of_literal "### RSA: Failure\n\n");
   C.EXIT_SUCCESS
